Source/Dafny/Translator.cs
@@ -9963,9 +9963,6 @@ namespace Microsoft.Dafny {
       if (exists.Bounds != null) {
         ex.Bounds = exists.Bounds.ConvertAll(bound => s.SubstituteBoundedPool(bound));
       }
-      if (exists.MissingBounds != null) {
-        ex.MissingBounds = exists.MissingBounds.ConvertAll(bv => var4var[bv]);
-      }
       return ex;
     }
 
@@ -17030,20 +17027,26 @@ namespace Microsoft.Dafny {
           return new ComprehensionExpr.IntBoundedPool(b.LowerBound == null ? null : Substitute(b.LowerBound), b.UpperBound == null ? null : Substitute(b.UpperBound));
         } else if (bound is ComprehensionExpr.SetBoundedPool) {
           var b = (ComprehensionExpr.SetBoundedPool)bound;
-          return new ComprehensionExpr.SetBoundedPool(Substitute(b.Set), b.ExactTypes);
+          return new ComprehensionExpr.SetBoundedPool(Substitute(b.Set), b.ExactTypes, b.IsFiniteCollection);
         } else if (bound is ComprehensionExpr.SubSetBoundedPool) {
           var b = (ComprehensionExpr.SubSetBoundedPool)bound;
-          return new ComprehensionExpr.SubSetBoundedPool(Substitute(b.UpperBound));
+          return new ComprehensionExpr.SubSetBoundedPool(Substitute(b.UpperBound), b.IsFiniteCollection);
         } else if (bound is ComprehensionExpr.SuperSetBoundedPool) {
           var b = (ComprehensionExpr.SuperSetBoundedPool)bound;
           return new ComprehensionExpr.SuperSetBoundedPool(Substitute(b.LowerBound));
         } else if (bound is ComprehensionExpr.MapBoundedPool) {
           var b = (ComprehensionExpr.MapBoundedPool)bound;
-          return new ComprehensionExpr.MapBoundedPool(Substitute(b.Map), b.ExactTypes);
+          return new ComprehensionExpr.MapBoundedPool(Substitute(b.Map), b.ExactTypes, b.IsFiniteCollection);
         } else if (bound is ComprehensionExpr.SeqBoundedPool) {
           var b = (ComprehensionExpr.SeqBoundedPool)bound;
           return new ComprehensionExpr.SeqBoundedPool(Substitute(b.Seq), b.ExactTypes);
         } else if (bound is ComprehensionExpr.DatatypeBoundedPool) {
+          return bound;  // nothing to substitute
+        } else if (bound is ComprehensionExpr.AllocFreeBoundedPool) {
+          return bound;  // nothing to substitute
+        } else if (bound is ComprehensionExpr.ExplicitAllocatedBoundedPool) {
+          return bound;  // nothing to substitute
+        } else if (bound is AssignSuchThatStmt.WiggleWaggleBound) {
           return bound;  // nothing to substitute
         } else {
           Contract.Assume(false);  // unexpected ComprehensionExpr.BoundedPool
